Added printf + better error messages + fixed ReprAST bugs (#372)
* Matched parentheses in ReprAST

* added fixed (?) ast

* Fixed vaargs not printing parens correctly

* removed duplicate large file

* Removed printf-ast per #370

* ast_printer now emits valid Coq code

* Fixed printing bugs.

* Gave ReprAst float conversion.

* Added complete terminator reprs (old todo)

* Added embedded printf definition as a .v.

* Slightly improved error message in interpreter.ml (old todo)

* Added putchar, merged builtins, better puts error messages.

* Added printf.

* Updated vaargs README

* Reorganized printf

* Fixed last ll files before merge

* Proof of putchar inf / fin in LangRefine.v

---------

Co-authored-by: Calvin Beck <hobbes@ualberta.ca>

src/ml/interpreter.ml
@@ -124,9 +124,11 @@ let rec step
   (* We finished the computation *)
   | RetF (_, (_, (_, (_, v)))) -> Ok v
   (* The ExternalCallE effect *)
-  | VisF (Sum.Coq_inl1 (ExternalCall (_, _, _)), _) ->
-      Error (UninterpretedCall "Uninterpreted Call")
-  (* TODO: More informative message *)
+  | VisF (Sum.Coq_inl1 (ExternalCall (t, _, dvs)), _) ->
+      Error (UninterpretedCall ("Call with return type " 
+       ^ (Camlcoq.camlstring_of_coqstring (ReprAST.repr_dtyp t))
+       ^ ", " ^ (string_of_int (List.length dvs)) ^ " dvalues."))
+  (* Still TODO: Integrate 2nd argument *)
   (* The IO_stdout effect *)
   | VisF (Sum.Coq_inl1 (IO_stdout bytes), k) ->
       let str = string_of_bytes bytes in
