src/ml/libvellvm/ast_printer.ml
@@ -6,11 +6,27 @@
 (*
   TODO: The ReprAST.repr_tle (and related "repr" type classes) stack overflow on large inputs.
 *)
-let toplevel_entities (fmt : Format.formatter) (tles: (LLVMAst.typ , (LLVMAst.typ LLVMAst.block) * ((LLVMAst.typ LLVMAst.block) list)) LLVMAst.toplevel_entities) : unit =
+(* let toplevel_entities (fmt : Format.formatter) (tles: (LLVMAst.typ , (LLVMAst.typ LLVMAst.block) * ((LLVMAst.typ LLVMAst.block) list)) LLVMAst.toplevel_entities) : unit =
   List.iter
     (fun tle ->
        Format.pp_print_string fmt (Camlcoq.camlstring_of_coqstring (ReprAST.repr_tle tle)))
-    tles
+    tles *)
 
+let toplevel_entities (fmt : Format.formatter) (tles: (LLVMAst.typ , (LLVMAst.typ LLVMAst.block) * ((LLVMAst.typ LLVMAst.block) list)) LLVMAst.toplevel_entities) : unit =
+  (* list formatting so the resulting term is valid *)
+  let print_list f lst =
+    let rec print_elements = function
+      | []   -> ()
+      | [h]  -> f h
+      | h::t -> f h; Format.pp_print_string fmt ";"; print_elements t
+    in
+    Format.pp_print_string fmt "[";
+    print_elements lst;
+    Format.pp_print_string fmt "]"
+  in 
+  print_list
+  (fun tle ->
+      Format.pp_print_string fmt (Camlcoq.camlstring_of_coqstring (ReprAST.repr_tle tle)))
+      tles
 
 
