utilities/vaargs/tests/raw-printf-usage/printf-many-types.ll
@@ -1,17 +1,23 @@
-; ModuleID = 'printf-no-vaargs.c'
-source_filename = "printf-no-vaargs.c"
+; ModuleID = 'printf-many-types.c'
+source_filename = "printf-many-types.c"
 target datalayout = "e-m:o-i64:64-i128:128-n32:64-S128"
 target triple = "arm64-apple-macosx14.0.0"
 
-@.str = private unnamed_addr constant [13 x i8] c"Hello world\0A\00", align 1
+@.str = private unnamed_addr constant [38 x i8] c"In C, %d can be %c or %x or even %o.\0A\00", align 1
 
 ; Function Attrs: noinline nounwind optnone ssp uwtable
-define void @printf_helloworld() #0 {
-  %1 = call i32 (i8*, ...) @printf(i8* noundef getelementptr inbounds ([13 x i8], [13 x i8]* @.str, i64 0, i64 0))
+define void @printf_polymorphism_for_free() #0 {
+  %1 = call i32 (i8*, ...) @printf(i8* noundef getelementptr inbounds ([38 x i8], [38 x i8]* @.str, i64 0, i64 0), i32 noundef 48, i32 noundef 48, i32 noundef 48, i32 noundef 48)
   ret void
 }
 
 declare i32 @printf(i8* noundef, ...) #1
+
+; Function Attrs: noinline nounwind optnone ssp uwtable
+define i32 @main() #0 {
+  call void @printf_polymorphism_for_free()
+  ret i32 0
+}
 
 attributes #0 = { noinline nounwind optnone ssp uwtable "frame-pointer"="non-leaf" "min-legal-vector-width"="0" "no-trapping-math"="true" "stack-protector-buffer-size"="8" "target-cpu"="apple-m1" "target-features"="+aes,+crc,+crypto,+dotprod,+fp-armv8,+fp16fml,+fullfp16,+lse,+neon,+ras,+rcpc,+rdm,+sha2,+v8.5a,+zcm,+zcz" }
 attributes #1 = { "frame-pointer"="non-leaf" "no-trapping-math"="true" "stack-protector-buffer-size"="8" "target-cpu"="apple-m1" "target-features"="+aes,+crc,+crypto,+dotprod,+fp-armv8,+fp16fml,+fullfp16,+lse,+neon,+ras,+rcpc,+rdm,+sha2,+v8.5a,+zcm,+zcz" }
