utilities/vaargs/tests/raw-printf-usage/printf-nested.ll
@@ -1,17 +1,26 @@
-; ModuleID = 'printf-one-vaarg.c'
-source_filename = "printf-one-vaarg.c"
+; ModuleID = 'printf-nested.c'
+source_filename = "printf-nested.c"
 target datalayout = "e-m:o-i64:64-i128:128-n32:64-S128"
 target triple = "arm64-apple-macosx14.0.0"
 
-@.str = private unnamed_addr constant [76 x i8] c"We gotta find out which cell this princess of yours is in. Here it is. %d.\0A\00", align 1
+@.str = private unnamed_addr constant [55 x i8] c"The string was %s, the number of chars printed is %d.\0A\00", align 1
+@.str.1 = private unnamed_addr constant [12 x i8] c"Oh hi there\00", align 1
+@.str.2 = private unnamed_addr constant [13 x i8] c"Oh hi there!\00", align 1
 
 ; Function Attrs: noinline nounwind optnone ssp uwtable
-define void @printf_solo() #0 {
-  %1 = call i32 (i8*, ...) @printf(i8* noundef getelementptr inbounds ([76 x i8], [76 x i8]* @.str, i64 0, i64 0), i32 noundef 2187)
+define void @printf_infiniti() #0 {
+  %1 = call i32 (i8*, ...) @printf(i8* noundef getelementptr inbounds ([13 x i8], [13 x i8]* @.str.2, i64 0, i64 0))
+  %2 = call i32 (i8*, ...) @printf(i8* noundef getelementptr inbounds ([55 x i8], [55 x i8]* @.str, i64 0, i64 0), i8* noundef getelementptr inbounds ([12 x i8], [12 x i8]* @.str.1, i64 0, i64 0), i32 noundef %1)
   ret void
 }
 
 declare i32 @printf(i8* noundef, ...) #1
+
+; Function Attrs: noinline nounwind optnone ssp uwtable
+define i32 @main() #0 {
+  call void @printf_infiniti()
+  ret i32 0
+}
 
 attributes #0 = { noinline nounwind optnone ssp uwtable "frame-pointer"="non-leaf" "min-legal-vector-width"="0" "no-trapping-math"="true" "stack-protector-buffer-size"="8" "target-cpu"="apple-m1" "target-features"="+aes,+crc,+crypto,+dotprod,+fp-armv8,+fp16fml,+fullfp16,+lse,+neon,+ras,+rcpc,+rdm,+sha2,+v8.5a,+zcm,+zcz" }
 attributes #1 = { "frame-pointer"="non-leaf" "no-trapping-math"="true" "stack-protector-buffer-size"="8" "target-cpu"="apple-m1" "target-features"="+aes,+crc,+crypto,+dotprod,+fp-armv8,+fp16fml,+fullfp16,+lse,+neon,+ras,+rcpc,+rdm,+sha2,+v8.5a,+zcm,+zcz" }
