utilities/vaargs/tests/raw-printf-usage/printf-no-vaargs.c
@@ -1,3 +1,7 @@
 void printf_helloworld() {
     printf("Hello world\n");
 }
+
+int main() {
+    printf_helloworld();
+}
