utilities/vaargs/tests/with-linking/main.ll
@@ -1,0 +1,30 @@
+; ModuleID = 'main.c'
+source_filename = "main.c"
+target datalayout = "e-m:o-i64:64-i128:128-n32:64-S128"
+target triple = "arm64-apple-macosx14.0.0"
+
+; Function Attrs: noinline nounwind optnone ssp uwtable
+define i32 @main(i32 noundef %0, i8** noundef %1) #0 {
+  %3 = alloca i32, align 4
+  %4 = alloca i32, align 4
+  %5 = alloca i8**, align 8
+  store i32 0, i32* %3, align 4
+  store i32 %0, i32* %4, align 4
+  store i8** %1, i8*** %5, align 8
+  ret i32 0
+}
+
+attributes #0 = { noinline nounwind optnone ssp uwtable "frame-pointer"="non-leaf" "min-legal-vector-width"="0" "no-trapping-math"="true" "stack-protector-buffer-size"="8" "target-cpu"="apple-m1" "target-features"="+aes,+crc,+crypto,+dotprod,+fp-armv8,+fp16fml,+fullfp16,+lse,+neon,+ras,+rcpc,+rdm,+sha2,+v8.5a,+zcm,+zcz" }
+
+!llvm.module.flags = !{!0, !1, !2, !3, !4, !5, !6, !7}
+!llvm.ident = !{!8}
+
+!0 = !{i32 1, !"wchar_size", i32 4}
+!1 = !{i32 1, !"branch-target-enforcement", i32 0}
+!2 = !{i32 1, !"sign-return-address", i32 0}
+!3 = !{i32 1, !"sign-return-address-all", i32 0}
+!4 = !{i32 1, !"sign-return-address-with-bkey", i32 0}
+!5 = !{i32 7, !"PIC Level", i32 2}
+!6 = !{i32 7, !"uwtable", i32 1}
+!7 = !{i32 7, !"frame-pointer", i32 1}
+!8 = !{!"Homebrew clang version 14.0.6"}
